\documentclass[12pt]{article}

\usepackage{amssymb,amsmath,amsthm}
\usepackage{bm}
\usepackage{graphicx,subcaption}
\usepackage[letterpaper, top=1in, left=1in, right=1in, bottom=1in]{geometry}

\newtheorem{definition}{Definition}
\newtheorem{theorem}{Theorem}
\newtheorem{lemma}{Lemma}
\newtheorem{remark}{Remark}

\newcommand{\SO}{\ensuremath{\mathrm{SO}(3)}}
\newcommand{\tr}[1]{\ensuremath{\mathrm{tr}\left( #1 \right)}}
\newcommand{\abs}[1]{\ensuremath{\left| #1 \right|}}

\title{\vspace{-4ex}\textbf{Product rule for FFT on SO(3)\vspace{-4ex}}}
\date{}

\begin{document}

\maketitle

Let $f,g\in L^2(\SO)$, $F_{m,n}^l$, $G_{m,n}^l$ be the corresponding Fourier coefficients for $0\leq l \leq B-1$ and $-l\leq m,n\leq l$.
Then we have the approximation
\begin{align*}
	f(R) = \sum_{l=0}^{B-1} \sum_{m,n=-l}^l (2l+1) F_{m,n}^l D_{m,n}^l(R) \\
	g(R) = \sum_{l=0}^{B-1} \sum_{m,n=-l}^l (2l+2) G_{m,n}^l D_{m,n}^l(R).
\end{align*}
The product of $f$ and $g$ has approximation
\begin{align*}
	(fg)(R) &= \sum_{l_1=0}^{B-1} \sum_{l_2=0}^{B-1} \sum_{m_1,n_1=-l_1}^{l_1} \sum_{m_2,n_2=-l_2}^{l_2} (2l_1+1)(2l_2+1) F_{m_1,n_1}^{l_1} G_{m_2,n_2}^{l_2} D_{m_1,n_1}^{l_1}(R) D_{m_2,n_2}^{l_2}(R) \\
	&= \sum_{l_1=0}^{B-1} \sum_{l_2=0}^{B-1} (2l_1+1)(2l_2+1) \tr{F^{l_1} \otimes G^{l_2} \cdot \left(D^{l_1}(R) \otimes D^{l_2}(R)\right)^T} \\
	&= \sum_{l_1=0}^{B-1} \sum_{l_2=0}^{B-1} (2l_1+1)(2l_2+1) \tr{C_{l_1,l_2}^T F^{l_1} \otimes G^{l_2} C_{l_1,l_2} \bigoplus_{l=\abs{l_1-l_2}}^{l_1+l_2} D^l(R)^T},
\end{align*}
where $C_{l_1,l_2}$ is the Clebsch-Gordan coefficient. 
Let
\begin{align*}
	A_{l_1,l_2} = (2l_1+1)(2l_2+1) C_{l_1,l_2}^T F^{l_1} \otimes G^{l_2} C_{l_1,l_2},
\end{align*}
and denote the Fourier coefficients of $fg$ as $H_{m,n}^l$, then
\begin{align*}
	H^l = \sum_{\substack{\abs{l_1-l_2} \leq l \leq l_1+l_2 \\ 0 \leq l_1 \leq B-1 \\ 0 \leq l_2 \leq B-1}} = \frac{1}{2l+1} A_{l_1,l_2}(l),
\end{align*}
where $A_{l_1,l_2}(l)$ is a sub-diagonal block of $A_{l_1,l_2}$, whose row and column indices range from $l^2-(l_1-l_2)^2+1$ to $l^2-(l_1-l_2)^2+2l+1$.


\end{document}

